theories/zoo_saturn/queue_mpmc_2__code.v
@@ -1,0 +1,304 @@
+Require Import zoo.prelude.
+Require Import zoo.language.typeclasses.
+Require Import zoo.language.notations.
+Require Import zoo_std.domain.
+Require Import zoo.options.
+
+Notation "'queue_mpmc_2٠Front'" := (
+  in_type "zoo_saturn.queue_mpmc_2.suffix" 0
+)(in custom zoo_tag
+).
+Notation "'queue_mpmc_2٠Cons'" := (
+  in_type "zoo_saturn.queue_mpmc_2.suffix" 1
+)(in custom zoo_tag
+).
+
+Notation "'queue_mpmc_2٠Back'" := (
+  in_type "zoo_saturn.queue_mpmc_2.prefix" 0
+)(in custom zoo_tag
+).
+Notation "'queue_mpmc_2٠Snoc'" := (
+  in_type "zoo_saturn.queue_mpmc_2.prefix" 1
+)(in custom zoo_tag
+).
+Notation "'queue_mpmc_2٠Used'" := (
+  in_type "zoo_saturn.queue_mpmc_2.prefix" 2
+)(in custom zoo_tag
+).
+
+Notation "'queue_mpmc_2٠index'" := (
+  in_type "zoo_saturn.queue_mpmc_2.prefix.Back" 0
+)(in custom zoo_field
+).
+Notation "'queue_mpmc_2٠move'" := (
+  in_type "zoo_saturn.queue_mpmc_2.prefix.Back" 1
+)(in custom zoo_field
+).
+
+Notation "'queue_mpmc_2٠front'" := (
+  in_type "zoo_saturn.queue_mpmc_2.t" 0
+)(in custom zoo_field
+).
+Notation "'queue_mpmc_2٠back'" := (
+  in_type "zoo_saturn.queue_mpmc_2.t" 1
+)(in custom zoo_field
+).
+
+Definition queue_mpmc_2٠suffix_index : val :=
+  𝗳𝘂𝗻 "suff" ->
+    𝗺𝗮𝘁𝗰𝗵 "suff" 𝘄𝗶𝘁𝗵
+    | queue_mpmc_2٠Front "i" ->
+        "i"
+    | queue_mpmc_2٠Cons "i" ⎽ ⎽ ->
+        "i"
+    𝗲𝗻𝗱.
+
+Definition queue_mpmc_2٠prefix_index : val :=
+  𝗳𝘂𝗻 "pref" ->
+    𝗺𝗮𝘁𝗰𝗵 "pref" 𝘄𝗶𝘁𝗵
+    | queue_mpmc_2٠Back ⎽ ⎽ 𝗮𝘀 "back_r" ->
+        "back_r".{queue_mpmc_2٠index}
+    | queue_mpmc_2٠Snoc "i" ⎽ ⎽ ->
+        "i"
+    𝗲𝗻𝗱.
+
+Definition queue_mpmc_2٠rev₁ : val :=
+  𝗿𝗲𝗰 "rev" "suff" "pref" ->
+    𝗺𝗮𝘁𝗰𝗵 "suff" 𝘄𝗶𝘁𝗵
+    | queue_mpmc_2٠Cons ⎽ ⎽ ⎽ 𝗮𝘀 "suff" ->
+        𝗺𝗮𝘁𝗰𝗵 "pref" 𝘄𝗶𝘁𝗵
+        | queue_mpmc_2٠Back ⎽ ⎽ ->
+            "suff"
+        | queue_mpmc_2٠Snoc "i" "v" "pref" ->
+            "rev" ‘queue_mpmc_2٠Cons[ "i", "v", "suff" ] "pref"
+        𝗲𝗻𝗱
+    𝗲𝗻𝗱.
+
+Definition queue_mpmc_2٠rev : val :=
+  𝗳𝘂𝗻 "back" ->
+    𝗺𝗮𝘁𝗰𝗵 "back" 𝘄𝗶𝘁𝗵
+    | queue_mpmc_2٠Snoc "i" "v" "pref" ->
+        queue_mpmc_2٠rev₁
+          ‘queue_mpmc_2٠Cons[ "i",
+            "v",
+            ‘queue_mpmc_2٠Front[ "i" + 1 ]
+          ]
+          "pref"
+    𝗲𝗻𝗱.
+
+Definition queue_mpmc_2٠create : val :=
+  𝗳𝘂𝗻 ⎽ ->
+    { ‘queue_mpmc_2٠Front[ 1 ],
+      ‘queue_mpmc_2٠Back{ 0, §queue_mpmc_2٠Used }
+    }.
+
+Definition queue_mpmc_2٠size : val :=
+  𝗿𝗲𝗰 "size" "t" ->
+    𝗹𝗲𝘁 "front" = "t".{queue_mpmc_2٠front} 𝗶𝗻
+    𝗹𝗲𝘁 "proph" = 𝗽𝗿𝗼𝗽𝗵 𝗶𝗻
+    𝗹𝗲𝘁 "back" = "t".{queue_mpmc_2٠back} 𝗶𝗻
+    𝗶𝗳
+      𝗹𝗲𝘁 "@tmp" = "t".{queue_mpmc_2٠front} == "front" 𝗶𝗻
+      𝗿𝗲𝘀𝗼𝗹𝘃𝗲 𝘀𝗸𝗶𝗽 "proph" "@tmp" ⍮
+      "@tmp"
+    𝘁𝗵𝗲𝗻 (
+      queue_mpmc_2٠prefix_index "back" - queue_mpmc_2٠suffix_index "front"
+      +
+      1
+    ) 𝗲𝗹𝘀𝗲 (
+      "size" "t"
+    ).
+
+Definition queue_mpmc_2٠is_empty : val :=
+  𝗳𝘂𝗻 "t" ->
+    queue_mpmc_2٠size "t" == 0.
+
+Definition queue_mpmc_2٠finish : val :=
+  𝗳𝘂𝗻 "back" ->
+    𝗺𝗮𝘁𝗰𝗵 "back" 𝘄𝗶𝘁𝗵
+    | queue_mpmc_2٠Back ⎽ ⎽ 𝗮𝘀 "back_r" ->
+        "back_r" <-{queue_mpmc_2٠move} §queue_mpmc_2٠Used
+    𝗲𝗻𝗱.
+
+Definition queue_mpmc_2٠help : val :=
+  𝗳𝘂𝗻 "t" "back" "i_move" "move" ->
+    𝗺𝗮𝘁𝗰𝗵 "t".{queue_mpmc_2٠front} 𝘄𝗶𝘁𝗵
+    | queue_mpmc_2٠Front "i_front" 𝗮𝘀 "front" ->
+        𝗶𝗳
+          "i_move" < "i_front"
+          𝗼𝗿
+          𝗰𝗮𝘀
+            "t".[queue_mpmc_2٠front]
+            "front"
+            (queue_mpmc_2٠rev "move")
+        𝘁𝗵𝗲𝗻 (
+          queue_mpmc_2٠finish "back"
+        )
+    | ⎽ ->
+        queue_mpmc_2٠finish "back"
+    𝗲𝗻𝗱.
+
+#[local] Definition __zoo_recs_0 :=
+  ( 𝗿𝗲𝗰𝘀 "push_aux" "t" "v" "i" "back" ->
+      𝗹𝗲𝘁 "new_back" =
+        ‘queue_mpmc_2٠Snoc[ "i" + 1, "v", "back" ]
+      𝗶𝗻
+      𝗶𝗳
+        ~ 𝗰𝗮𝘀 "t".[queue_mpmc_2٠back] "back" "new_back"
+      𝘁𝗵𝗲𝗻 (
+        domain٠yield () ⍮
+        "push" "t" "v"
+      )
+    𝘄𝗶𝘁𝗵 "push" "t" "v" ->
+      𝗺𝗮𝘁𝗰𝗵 "t".{queue_mpmc_2٠back} 𝘄𝗶𝘁𝗵
+      | queue_mpmc_2٠Snoc "i" ⎽ ⎽ 𝗮𝘀 "back" ->
+          "push_aux" "t" "v" "i" "back"
+      | queue_mpmc_2٠Back ⎽ ⎽ 𝗮𝘀 "back" ->
+          𝗹𝗲𝘁 "back_r" = "back" 𝗶𝗻
+          𝗺𝗮𝘁𝗰𝗵 "back_r".{queue_mpmc_2٠move} 𝘄𝗶𝘁𝗵
+          | queue_mpmc_2٠Used ->
+              "push_aux" "t" "v" "back_r".{queue_mpmc_2٠index} "back"
+          | queue_mpmc_2٠Snoc "i_move" ⎽ ⎽ 𝗮𝘀 "move" ->
+              queue_mpmc_2٠help "t" "back" "i_move" "move" ⍮
+              "push" "t" "v"
+          𝗲𝗻𝗱
+      𝗲𝗻𝗱
+  )%zoo_recs.
+Definition queue_mpmc_2٠push_aux :=
+  ValRecs 0 __zoo_recs_0.
+Definition queue_mpmc_2٠push :=
+  ValRecs 1 __zoo_recs_0.
+#[global] Instance :
+  AsValRecs' queue_mpmc_2٠push_aux 0 __zoo_recs_0 [
+    queue_mpmc_2٠push_aux ;
+    queue_mpmc_2٠push
+  ].
+Proof.
+  done.
+Qed.
+#[global] Instance :
+  AsValRecs' queue_mpmc_2٠push 1 __zoo_recs_0 [
+    queue_mpmc_2٠push_aux ;
+    queue_mpmc_2٠push
+  ].
+Proof.
+  done.
+Qed.
+
+#[local] Definition __zoo_recs_1 :=
+  ( 𝗿𝗲𝗰𝘀 "pop_1" "t" "front" ->
+      𝗺𝗮𝘁𝗰𝗵 "front" 𝘄𝗶𝘁𝗵
+      | queue_mpmc_2٠Cons ⎽ "v" "new_front" ->
+          𝗶𝗳
+            𝗰𝗮𝘀 "t".[queue_mpmc_2٠front] "front" "new_front"
+          𝘁𝗵𝗲𝗻 (
+            ‘Some( "v" )
+          ) 𝗲𝗹𝘀𝗲 (
+            domain٠yield () ⍮
+            "pop" "t"
+          )
+      | queue_mpmc_2٠Front "i_front" 𝗮𝘀 "front" ->
+          𝗺𝗮𝘁𝗰𝗵 "t".{queue_mpmc_2٠back} 𝘄𝗶𝘁𝗵
+          | queue_mpmc_2٠Snoc "i_move" "v" "move_pref" 𝗮𝘀 "move" ->
+              𝗶𝗳 "i_front" == "i_move" 𝘁𝗵𝗲𝗻 (
+                𝗶𝗳
+                  𝗰𝗮𝘀 "t".[queue_mpmc_2٠back] "move" "move_pref"
+                𝘁𝗵𝗲𝗻 (
+                  ‘Some( "v" )
+                ) 𝗲𝗹𝘀𝗲 (
+                  "pop" "t"
+                )
+              ) 𝗲𝗹𝘀𝗲 (
+                𝗺𝗮𝘁𝗰𝗵
+                  ‘queue_mpmc_2٠Back{ "i_move", "move" }
+                𝘄𝗶𝘁𝗵
+                | queue_mpmc_2٠Back ⎽ ⎽ 𝗮𝘀 "back" ->
+                    𝗹𝗲𝘁 "front'" =
+                      "t".{queue_mpmc_2٠front}
+                    𝗶𝗻
+                    𝗶𝗳 "front'" != "front" 𝘁𝗵𝗲𝗻 (
+                      "pop_1" "t" "front'"
+                    ) 𝗲𝗹𝘀𝗲 𝗶𝗳
+                       𝗰𝗮𝘀 "t".[queue_mpmc_2٠back] "move" "back"
+                     𝘁𝗵𝗲𝗻 (
+                      "pop_2" "t" "front" "back" "move"
+                    ) 𝗲𝗹𝘀𝗲 (
+                      "pop" "t"
+                    )
+                𝗲𝗻𝗱
+              )
+          | queue_mpmc_2٠Back ⎽ ⎽ ->
+              "pop_3" "t" "front"
+          𝗲𝗻𝗱
+      𝗲𝗻𝗱
+    𝘄𝗶𝘁𝗵 "pop_2" "t" "front" "back" "move" ->
+      𝗺𝗮𝘁𝗰𝗵 queue_mpmc_2٠rev "move" 𝘄𝗶𝘁𝗵
+      | queue_mpmc_2٠Cons ⎽ "v" "new_front" ->
+          𝗶𝗳
+            𝗰𝗮𝘀 "t".[queue_mpmc_2٠front] "front" "new_front"
+          𝘁𝗵𝗲𝗻 (
+            queue_mpmc_2٠finish "back" ⍮
+            ‘Some( "v" )
+          ) 𝗲𝗹𝘀𝗲 (
+            domain٠yield () ⍮
+            "pop" "t"
+          )
+      𝗲𝗻𝗱
+    𝘄𝗶𝘁𝗵 "pop_3" "t" "front" ->
+      𝗹𝗲𝘁 "front'" = "t".{queue_mpmc_2٠front} 𝗶𝗻
+      𝗶𝗳 "front'" == "front" 𝘁𝗵𝗲𝗻 (
+        §None
+      ) 𝗲𝗹𝘀𝗲 (
+        "pop_1" "t" "front'"
+      )
+    𝘄𝗶𝘁𝗵 "pop" "t" ->
+      "pop_1" "t" "t".{queue_mpmc_2٠front}
+  )%zoo_recs.
+Definition queue_mpmc_2٠pop_1 :=
+  ValRecs 0 __zoo_recs_1.
+Definition queue_mpmc_2٠pop_2 :=
+  ValRecs 1 __zoo_recs_1.
+Definition queue_mpmc_2٠pop_3 :=
+  ValRecs 2 __zoo_recs_1.
+Definition queue_mpmc_2٠pop :=
+  ValRecs 3 __zoo_recs_1.
+#[global] Instance :
+  AsValRecs' queue_mpmc_2٠pop_1 0 __zoo_recs_1 [
+    queue_mpmc_2٠pop_1 ;
+    queue_mpmc_2٠pop_2 ;
+    queue_mpmc_2٠pop_3 ;
+    queue_mpmc_2٠pop
+  ].
+Proof.
+  done.
+Qed.
+#[global] Instance :
+  AsValRecs' queue_mpmc_2٠pop_2 1 __zoo_recs_1 [
+    queue_mpmc_2٠pop_1 ;
+    queue_mpmc_2٠pop_2 ;
+    queue_mpmc_2٠pop_3 ;
+    queue_mpmc_2٠pop
+  ].
+Proof.
+  done.
+Qed.
+#[global] Instance :
+  AsValRecs' queue_mpmc_2٠pop_3 2 __zoo_recs_1 [
+    queue_mpmc_2٠pop_1 ;
+    queue_mpmc_2٠pop_2 ;
+    queue_mpmc_2٠pop_3 ;
+    queue_mpmc_2٠pop
+  ].
+Proof.
+  done.
+Qed.
+#[global] Instance :
+  AsValRecs' queue_mpmc_2٠pop 3 __zoo_recs_1 [
+    queue_mpmc_2٠pop_1 ;
+    queue_mpmc_2٠pop_2 ;
+    queue_mpmc_2٠pop_3 ;
+    queue_mpmc_2٠pop
+  ].
+Proof.
+  done.
+Qed.
