theories/zoo_saturn/queue_mpmc_2__types.v
@@ -5,41 +5,41 @@ Require Export zoo_std.domain.
 Require Import zoo.options.
 
 Notation "'Front'" := (
-  in_type "zoo_saturn.mpmc_queue_2.suffix" 0
+  in_type "zoo_saturn.queue_mpmc_2.suffix" 0
 )(in custom zoo_tag
 ).
 Notation "'Cons'" := (
-  in_type "zoo_saturn.mpmc_queue_2.suffix" 1
+  in_type "zoo_saturn.queue_mpmc_2.suffix" 1
 )(in custom zoo_tag
 ).
 
 Notation "'Back'" := (
-  in_type "zoo_saturn.mpmc_queue_2.prefix" 0
+  in_type "zoo_saturn.queue_mpmc_2.prefix" 0
 )(in custom zoo_tag
 ).
 Notation "'Snoc'" := (
-  in_type "zoo_saturn.mpmc_queue_2.prefix" 1
+  in_type "zoo_saturn.queue_mpmc_2.prefix" 1
 )(in custom zoo_tag
 ).
 Notation "'Used'" := (
-  in_type "zoo_saturn.mpmc_queue_2.prefix" 2
+  in_type "zoo_saturn.queue_mpmc_2.prefix" 2
 )(in custom zoo_tag
 ).
 
 Notation "'index'" := (
-  in_type "zoo_saturn.mpmc_queue_2.prefix.Back" 0
+  in_type "zoo_saturn.queue_mpmc_2.prefix.Back" 0
 )(in custom zoo_field
 ).
 Notation "'move'" := (
-  in_type "zoo_saturn.mpmc_queue_2.prefix.Back" 1
+  in_type "zoo_saturn.queue_mpmc_2.prefix.Back" 1
 )(in custom zoo_field
 ).
 
 Notation "'front'" := (
-  in_type "zoo_saturn.mpmc_queue_2.t" 0
+  in_type "zoo_saturn.queue_mpmc_2.t" 0
 )(in custom zoo_field
 ).
 Notation "'back'" := (
-  in_type "zoo_saturn.mpmc_queue_2.t" 1
+  in_type "zoo_saturn.queue_mpmc_2.t" 1
 )(in custom zoo_field
 ).
